src/regular/regex_from_dfa.lean
@@ -1,0 +1,47 @@
+import tactic
+import languages.basic
+import languages.star
+import regular.regex
+import automata.dfa
+
+open languages regex dfa
+
+namespace regex.from_dfa
+
+variables {S Q : Type} [fintype S] [fintype Q]
+
+inductive go_restr (dfa : DFA S Q) (allow : finset Q) : Q → list S → Q → Prop
+| finish {q : Q}                : go_restr q [] q
+| last_step {ch : S} {q : Q}    : go_restr q [ch] (dfa.next q ch)
+| step {head : S} {tail : list S} {q nxt f : Q} :
+    nxt = dfa.next q head → nxt ∈ allow → go_restr nxt tail f → go_restr q (head::tail) f
+
+lemma go_restr_univ (dfa : DFA S Q) {a b : Q} {w : list S}
+    : go dfa a w b ↔ go_restr dfa (fintype.elems Q) a w b :=
+begin
+    split, {
+        intro go_dfa,
+        induction go_dfa, 
+        { exact go_restr.finish }, 
+        { refine go_restr.step rfl (finset.mem_univ _) go_dfa_ih, }
+    }, {
+        intro go_restr_dfa,
+        induction go_restr_dfa, 
+        { exact go.finish },
+        { refine go.step go.finish },
+        { subst go_restr_dfa_a, refine go.step go_restr_dfa_ih },
+    }
+end
+
+def all_edges (dfa : DFA S Q) (a b : Q) : regex S := sorry
+
+def regex_from_to (dfa : DFA S Q) : Q → Q → finset Q → regex S := sorry
+-- | a b finset.empty := dfa_all_edges dfa a b,
+
+theorem dfa_to_regex {L : set (list S)} : dfa_lang L → regex_lang L :=
+begin
+    rintro ⟨Q, fQ, dfa, rfl⟩,
+    sorry,
+end
+
+end regex.from_dfa
